% Indicate the main file. Must go at the beginning of the file.
% !TEX root = ../main.tex

%%%%%%%%%%%%%%%%%%%%%%%%%%%%%%%%%%%%%%%%%%%%%%%%%%%%%%%%%%%%%%%%%%%%%%%%%%%%%%%%
% SECTION 2
%%%%%%%%%%%%%%%%%%%%%%%%%%%%%%%%%%%%%%%%%%%%%%%%%%%%%%%%%%%%%%%%%%%%%%%%%%%%%%%%

\section{Materials and Methods}
\label{section2}
\kant[14-15]
\begin{align*}
C(x) &= C_1(x) + C_2(x) \\
&= A_1e^{-\lambda_1 x} + A_2e^{-\lambda_2 (a-x)}
\end{align*}
\kant[19]\vspace{-0.5cm}
\begin{align*}
C'(x) &= -A_1\lambda_1 e^{-\lambda_1 x} + A_2 \lambda_2 e^{-\lambda_2 (a-x)} \stackrel{!}{=} 0\\
 &= -A_1\lambda_1 e^{-\lambda_1 x} + A_2 \lambda_2 e^{-\lambda_2 a} e^{\lambda_2 x} && | \cdot e^{+\lambda_1 x}\\
 &= -A_1\lambda_1 + A_2 \lambda_2 e^{-\lambda_2 a} e^{x (\lambda_1+\lambda_2)} && | \text{ rearrange...} \\
 e^{x(\lambda_1+\lambda_2)} &= \frac{A_1\lambda_1}{A_2\lambda_2}\cdot e^{\lambda_2 a} &&|\ln(\cdot)\\
x(\lambda_1 + \lambda_2) &= \ln\left(\frac{A_1\lambda_1}{A_2\lambda_2}\cdot e^{\lambda_2 a}\right)\\
 &= \ln\left(\frac{A_1\lambda_1}{A_2\lambda_2}\right) + \lambda_2 a \\
 &= \ln(A_1) + \ln(\lambda_1) - \ln(A_2) - \ln(\lambda_2) + \lambda_2 a
\end{align*}


\subsection{Clinical data}
\kant[14-16]
\subsection{Analysis}
\kant[45]
\begin{align*}
C(x) &= C_1(x) + C_2(x) \\
&= A_1e^{-\lambda_1 x} + A_2e^{-\lambda_2 (a-x)}
\end{align*}

\kant[45]


